<?xml version="1.0" encoding="UTF-8"?>

<section xml:id="sec_fourth-examplesC" xmlns:xi="http://www.w3.org/2001/XInclude">
  <title>Examples C</title>
  
<example>
  <statement>
    <p>
      A 10-kg block lying on the horizontal surface is pulled by a force 
      F making an angle of <m>60^{o}</m> above the horizontal. The coefficient of 
      static friction between the block and the horizontal surface is 0.3 and the 
      coefficient of kinetic friction is 0.2. Draw the appropriate diagrams, 
      write the appropriate equations, and find the magnitude and direction of 
      the acceleration of the block when  
      <image source="ntwn1a.png" width="30%"> </image> 
      <ol marker="a.">
        <li>
          <m> F = 30 N,</m>
        </li>
        <li><m>F = 60 N,</m></li>
        <li><m>F = 90 N,</m></li>
        <li><m>F = 120 N.</m></li>
      </ol>
      </p>
  </statement>
  <solution>
    <p>
      Given: <m>m =  10 kg, \quad \theta = 60^{o}, \quad \mu_{s} = 0.3, \quad \mu_{k} = 0.2, \quad g = 9.8 m/s^{2}.</m>
      <image source="ntwn1b.png" width="30%"> </image> 
    </p>
    <p>
      Equations:
      <me>
        \sum F_{x} = F \cos\theta - f  =  m a_{x}
      </me>
      <me>
        \sum F_{y} = F \sin\theta - w + N  =  m a_{y}
      </me>
      <me>
        f  =  \mu N;
      </me>
      <me>
        w  =  m g	\quad \rightarrow \quad	w  =  98 N 
      </me>
     </p>
     <p>
      <ol marker="a.">
        <li>
         <m>F  = 30 N.</m> 
     In verticle direction, <m>a_{y} = 0,</m>
      <me>
        \therefore \quad	N + F \sin\theta -w = 72.02 N 
      </me>
      In horizontal direction, assume <m>a_x=0</m> then,
      <me>
       f= F\cos\theta = 30\times \cos(60) =15N.
      </me>
      and 
      <me>
        f_s=\mu_s N = 0.3\times 72.02 = 21.61 N
      </me>
      Since <m>f \lt f_{s},</m> static friction can keep the block at rest as assumed.
      Therefore, 	<m>a  =  0, \quad \theta_{a}  =  0.</m>
        </li>
        <li>
          <m>F = 60 N.</m>
          Assume 
          <me>
            a_{y} = 0, \longrightarrow	N = w - F \sin\theta = 46.04 N 
          </me>
          and 
          <me>
            a_{x} = 0,\longrightarrow	f  =  F \cos\theta =  30 N, \quad f_{s}  = \mu_{s} N  =  13.812 N
          </me>
         Since <m>f \gt f_{s},</m> static friction cannot keep the block at rest as assumed. 
         Therefore block slides and,
         <me>
          \mu =\mu_{k} = 0.2;\quad f  = \mu N = 9.208 N
         </me>
         <me>
          a_{x} = (F \cos\theta - f)/m  =  2.079 m/s^{2}
         </me>
         <me>
          \therefore a  =  2.08 m/s^{2}, \quad \theta_{a}  =  0.
         </me>
         </li>
         <li>
          <m>F = 90 N.</m>
          Assume <me>
            a_{y} = 0, \rightarrow	N = w - F \sin\theta = 20.058 N
          </me>
         Assume block slides, 
         <me>
          \mu = \mu_{s} = 0.2;\quad f  = \mu N = 4.099 N
         </me>
         <me>
          a_{x} = (F \cos\theta - f)/m  =  4.011 m/s^{2}\qquad \therefore a  =  4.01 m/s^{2},\quad \theta_{a}  =  0.
         </me>
         </li>
         <li>
          <m>F = 120 N.</m>
          Assume 
          <me>
            a_{y} = 0, \rightarrow	N = w - F \sin\theta =  - 5.923 N
          </me>
          Since N cannot be negative, our assumption was false and block leaves the surface.
          <me>
            \therefore,	N = 0,  \quad f  =  0;\quad a_{x} = (F \cos\theta)/m  =  6.000 m/s^{2}
          </me>
          <me>
            a_{y}  =  (F \sin\theta - w)/m  =  0.5923 m/s^{2} ; a  =  	=  6.029 m/s^{2}
          </me>
          <me>
            \tan\theta_{a}  = \frac{a_{y}}{a_{x}}  \rightarrow  \theta_{a} =  5.638^{o}
          </me>
          <me>
            \therefore, 	a  =  6.03 m/s^{2}, \quad \theta_{a}  =  5.64^{o}. 
          </me>
             </li>
      </ol>
     </p>
  </solution>
</example>

<example>
  <statement>
    <p>
      A block of mass <m>m_{1} = 10 kg </m> rests on top of a larger block of mass 
      <m>m_{2}</m> = 25 kg which rests on a plane inclined at an angle <m>\theta = 10^{o}</m>. 
      The coefficient of static friction between all surfaces is <m>0.3</m> and that of 
      kinetic friction is <m>0.2</m>. A constant force <m>F</m> parallel to the plane is 
      applied to <m>m_{2}</m>  accelerating it up the plane. 
      <image source="ntwn4.png" width="30%"> </image> 
      <ol marker="a.">
        <li>
          What is the maximum acceleration of <m>m_{2}</m>  which will allow <m>m_{1}</m> to stay with it? 
        </li>
        <li>What is the force <m>F</m> which causes this acceleration?</li>
      </ol>
     </p>
  </statement>
  <solution>
    <p>
      Given: <m>m_{1} =10 kg, \quad m_{2} =25 kg,\quad \theta=10^{o}, \quad \mu_{1}=0.3,\quad \mu_{2}=0.2,
        \quad g =9.8m/s^{2}.</m> 
    </p>
    <p>
      From figure,  <image source="ntwn4b.png" width="30%"> </image> we have -
      <men xml:id="eqn-nwtn1">
        \sum F_{x}=f_{1}-w_{1}\sin\theta=m_{1}a  
      </men>
      <me>
        \sum F_{y}=N_{1}-w_{1}\cos\theta=0 
      </me>
      <men xml:id="eqn-nwtn2">
        \text{or,}\quad N_{1}=w_{1}\cos\theta = m_{1}g\cos\theta =10\times 9.8\times\cos 10^{o} =96.5 N 
      </men>
      also,
      <men xml:id="eqn-nwtn3">
        f_{1}=\mu_{1}N_{1}=0.3\times 96.5 = 28.95 N
      </men>
     now from eqn.<xref ref="eqn-nwtn1"/>,
     <men xml:id="eqn-nwtn4">
      a =\frac{f_{1}-w_{1}\sin\theta}{m_{1}} = \frac{28.95-10\times9.8\times\sin 10^{o}}{10}= 1.193 m/s^{2} 
     </men>
   From figure, <image source="ntwn4a.png" width="30%"> </image> we have -
   <men xml:id="eqn-nwtn5">
    \sum F_{x}=F-f_{1}-f_{2}-w_{2}\sin\theta=m_{2}a 
   </men>
   <me>
    \sum F_{y}=N_{2}-N_{1}-w_{2}\cos\theta=0 
   </me>
   <me>
    \text{or,}\quad N_{2}=N_{1}+w_{2}\cos\theta 
   </me>
   
   <men xml:id="eqn-nwtn6">
    =96.5+25\times9.8\times\cos 10^{o}=337.79N
   </men>
     
 <men xml:id="eqn-nwtn7">
  \text{also,}\quad f_{2}=\mu_{2}N_{2}=0.2\times 337.79 = 67.56 N
 </men>
 <me>
  \therefore\quad F = f_{1}+f_{2}+w_{2}\sin\theta+m_{2}a 
 </me>
 <me>
  = 28.95+67.56+25\times 9.8\times\sin 10^{o}+25\times1.193 = 168.88 N 
 </me>
    </p>
  </solution>
</example>

<example>
  <statement>
    <p>
      A box of mass 100 kg is placed in the front end of the bed of a truck initially 
      at rest. The coefficient of static friction between box and truck bed is 0.4, 
      the coefficient of kinetic friction between box and truck bed is 0.25, 
      the bed of the truck is 2 m long and 1 m above the ground, and the truck accelerates 
      at a constant acceleration just fast enough to make the box start sliding. 
      <image source="ntwn2a.png" width="50%"> </image>
      <ol marker="a.">
        <li>
          What is the acceleration of the truck?
        </li>
        <li>
          What is the acceleration of the box?
          </li>
          <li>
            When does the box fall off the back of the truck?
          </li>
          <li>
            How far does the truck travel before the box falls off? 
          </li>
          <li>
            How fast is the box traveling when it falls off the truck? 
          </li>
          <li>
            How far from its starting point does the box hit the ground?
          </li>
      </ol>
      </p>
  </statement>
  <solution>
    <p>
      Given: <m> m = 100 kg,  \quad \mu_{s}  =  0.4,  \quad \mu_{k} = 0.25,  \quad  L  =  2 m, \quad y  =  1 m </m> 
      <sidebyside widths="30% 30%">
        <image source="ntwn2b.png"> </image>
        <image source="ntwn2c.png"> </image>
      </sidebyside>
        </p>
    <ol marker="a.">
      <li>
        <p>
           <me>
          \sum F_{x}  =  f  =  m a_{2};\quad \sum F_{y}  =  N  -  w  =  0
        </me>
        <me>
          \mu=0.4, \quad w  =  m g =980N,\quad \therefore	N  =  980 N 
        </me>
        <me>
          f  =  \mu N; \quad	f  =  392 N, \quad \mu  =  \mu_{s}, \quad \therefore\qquad	a_{2}  =  3.92 m/s^{2} 
        </me>
      </p>
         </li>
      <li>
        <p>
          <me>
            \mu  =  \mu_{k}  =  0.25;	\quad f  =  245 N;\quad  a_{1}  =  2.45 m/s^{2}
          </me>  
        </p>
        </li>
        <li>
          <p>
            <me>
              x_{1}  =  v_{o1} t  +  \frac{1}{2}a_{1} t^{2}; 	\quad v_{o1}  = 0; 	\quad L  =  x_{1} - x_{2} =  +  t^{2}
            </me>
            <me>
              x_{2}  =  v_{o2} t   +  \frac{1}{2}a_{2} t^{2};\quad	v_{o2}  = 0; \quad	t  =  =  1.65 s; \qquad x_{1}  = x_{2}  +  L 	
            </me>
          </p>
        </li>
        <li>
          <p>
            <me>
              x_{1}  =  \frac{1}{2}a_{1} t^{2}   =  5.33 m
            </me>
            
          </p>
        </li>
        <li>
          <p>
            <me>
              v_{2}  =  v_{o2}  +  a_{2} t;	v_{2}  = 4.04 m/s
            </me>
            
          </p>
        </li>
        <li>
          <p>
           <me>
              x_{3}  =  v_{2} t_{2}; 	t_{2}  = 0.452 s
            </me>
            <me>
              y  =  \frac{1}{2}g t_{2}^{2}; 	x_{3}  = 1.825 m
            </me>
            <me>
              x_{T}  =  x_{1}  + x_{3}; \quad	x_{T}  =  7.16 m
            </me>
              </p>
        </li>
    </ol>
  </solution>
</example>

<example>
  <statement>
    <p>
      Pulley A is fixed to the ceiling, pulley B is suspended by the string 
      whose one end is attached to the ceiling and another end is passing 
      over pulley B and holding the block 1 of mass <m>m_{1}</m> as shown in figure below. 
      The block 2 of mass <m>m_{2}</m> is hanging from the pulley B. 
      If the pulleys and strings are massless and the strings do not stretch. 
      What is the correct relationship between accelerations <m>a_{1}</m> and <m>a_{2}</m> of blocks 1 and 2? 
      <image source="pulley1b.png" width="30%"> </image>
    </p>
  </statement>
  <solution>
    <p>
      Since the pulleys are massless, tensions of each section of the string 
      in either side of pulleys are same as shown in figure. 
      <image source="pulley1c.png" width="50%"> </image>
      To find the relation between <m>a_{1}</m> and <m>a_{2}</m> add the lengths 
      of each section of the string and take its derivative as shown below. 
      Let <m>H</m> is the height of pulley A from reference level (ground level), 
      then length of string from pulley A to block 1 is given as <m>H-y_{1},</m> 
      length of section of string from pulley A to B is <m>H-y_{2}</m> and 
      length of section of string from pulley B to level of pulley A is <m>H-y_{2}</m>. 
    </p>
    <p>
      Ignore the lengths of string over pulleys and to the rest to ceiling. 
      It does not contribute any thing to the derivative of the length. Now
       <me>
        L=(H-y_{1})+(H-y_{2})+(H-y_{2}) = 3H -y_{1}-2y_{2}
       </me>
       where <m>y_{a}</m> and <m> y_{2}</m> are distances of block 1 
       and pulley B from the reference level, respectively. Since the string 
       does not stretch, we have -
       <me>
        \frac{\,dL}{\,dt} = 0 = 0 -\frac{\,dy_{1}}{\,dt} -2\frac{\,dy_{2}}{\,dt}
       </me>
       <me>
        \therefore \frac{\,dy_{1}}{\,dt} = -2\frac{\,dy_{2}}{\,dt} \quad \Rightarrow\quad v_{1}=-2v_{2}
       </me>
       That is velocity of block 1 <m>v_{1} </m> is just the double velocity of 
       block 2 <m> v_{2}</m> and negative sign indicates the velocity of block 
       2 is opposite to that of block 1. Again,
       <me>
        \frac{\,dv_{1}}{\,dt} = -2\frac{\,dv_{2}}{\,dt} 
       </me>
       <men xml:id="eqn-pulley1">
        \therefore a_{1}=-2a_{2} 
       </men>
     From free-body diagram, we have -
    <men xml:id="eqn-pulley2">
      m_{1}g-T=m_{1}a_{1}  \qquad \therefore\quad T=m_{1}g-m_{1}a_{1}   
    </men>
    <men xml:id="eqn-pulley3">
      \text{also}\quad T_{2}-m_{2} g = m_{2}a_{2}  \qquad \therefore\quad T_{2}=m_{2}g+m_{2}a_{2}    
    </men>
    <men xml:id="eqn-pulley4">
      \text{but}\quad T_{2} = T +T  \qquad \therefore \quad 2T = m_{2}g+m_{2}a_{2}  
    </men>
    <me>
      2\left[m_{1}g-m_{1}a_{1}\right] = m_{2}g+m_{2}a_{2} 
    </me>
    <me>
      \text{or,}\quad 2 m_{1}g -m_{2}g = m_{2}a_{2}+2m_{1}a_{1} 
    </me>
    <me>
      \text{or,}\quad \left(2 m_{1} -m_{2}\right) g = -m_{2}\frac{a_{1}}{2}+2m_{1}a_{1}  = a_{1}\left(2m_{1}-\frac{m_{2}}{2}\right)
    </me>
    <me>
      \therefore \quad a_{1} = \left[\frac{\left(2 m_{1} -m_{2}\right) g}{\left(2m_{1}-\frac{m_{2}}{2}\right)}\right] \qquad \text{and}\quad T = \frac{m_{1}m_{2}g}{4m_{1}-m_{2}} 
    </me>
    </p>
  </solution>
</example>

<example>
  <statement>
    <p>
      A 30 N force is applied at an angle of <m>37^{o} </m> to the horizontal 
      to move the two boxes attached to each other with a string. 
      If the force is applied on the box of mass 3kg and the mass of second box 
      is 1 kg, find the acceleration of the boxes and tension in the string. 
      Consider the kinetic friction between the surfaces of box and the road is 0.4.
      <image source="dynboxes.png" width="50%"> </image>
    </p>
  </statement>
  <solution>
    <p>
      Given: <m> \mu_{k}=0.4, \quad m_{1}=3 kg, \quad m_{2}=1 kg, \quad F=30N, \quad \theta=37^{o},</m> 
      and <m> g=9.8 m/s^{2}. </m> 
    </p>
    <p>
      From free body diagram, <image source="dynboxes1a.png" width="50%"> </image> we have -
      <men xml:id="eqn-dynbox1">
        \sum F_{x}=T-f_{2} =m_{2}a \qquad \Rightarrow\quad T=m_{2}a+f_{2}
      </men>
      <men xml:id="eqn-dynbox2">
        \sum F_{y}=N_{2}-m_{2}g =0 \qquad \Rightarrow\quad N_{2}=m_{2}g 
      </men>
      <men xml:id="eqn-dynbox3">
        \text{but,}\quad f_{2}=\mu_{k}N_{2}
      </men>
      <men xml:id="eqn-dynbox4">
        \therefore\quad T = m_{2}(a+\mu_{k}g) 
      </men>
    </p>
    <p>
        From free body diagram, <image source="dynboxes1b.png" width="50%"> </image> we have -
        <men xml:id="eqn-dynbox5">
          \sum F_{x}=F_{x}-T-f_{1} = m_{1}a \qquad \Rightarrow\quad T=F_{x} - m_{1}a-f_{1}
        </men>
        <men xml:id="eqn-dynbox6">
          \sum F_{y}=N_{1}+F_{y}-m_{1}g =0 \qquad \Rightarrow\quad N_{1}=m_{1}g -F_{y} 
        </men>
        <men xml:id="eqn-dynbox7">
          \text{but,}\quad f_{1}=\mu_{k}N_{1}
        </men>
        <men xml:id="eqn-dynbox8">
          \therefore\quad T = F\left(\cos\theta +\mu_{k}\sin\theta\right) -m_{1}(a+\mu_{k}g) 
        </men>
        On solving eqns. <xref ref="eqn-dynbox4"/> and <xref ref="eqn-dynbox8"/>, we have -
        <m>a=3.0 m/s^{2}</m> and <m>T=6.92 N.</m>
    </p>
  </solution>
</example>

</section>
