<?xml version="1.0" encoding="UTF-8"?>

<section xml:id="sec_sixth-intro" xmlns:xi="http://www.w3.org/2001/XInclude">
  <title>Newton's Law of Gravitation</title>
  
   <introduction>
    <figure xml:id="NLG1">
      <caption></caption>
      <image source="NLG1.png" width="40%"/>
  </figure>
    <p>
      Newton observed that when an object, such as an apple, was released near the surface of 
      the earth, it was accelerated toward the earth. Since the cause of such acceleration is 
      an unbalanced force, there must be a force pulling that object toward the earth. 
      On this basis he came up with an idea called  <term>Newton's Law of Universal Gravitation</term>. 
      It states that any two masses in the universe attract each other with a force that is 
      directly proportional to the product of the masses and inversely proportional to the 
      square of the distance between them. Mathematically, 
<me>
  F  \varpropto  \frac{m_{1}m_{2}}{r^{2}}
</me>
<me>
  \text{or,}\quad  F  =G \frac{m_{1}m_{2}}{r^{2}}
</me>
Where <m>m_{1}</m> and <m>m_{2}</m> are masses of two objects, <m>r</m> is the distance 
between them, and <m>G  =  6.67 \times 10^{-11} N.m^{2}/kg^{2}</m>, is the proportionality 
constant, also called the universal gravitational constant. The value of G was first 
measured by <em>Sir Henry Cavendish</em>  experimentally in 1798.  The force <m>F_{12}</m> 
is the force on mass 1 due to mass 2, the force <m> F_{21}</m> is the force on mass 
2 due to mass 1, and they are equal and opposite [<xref ref="NLG1"/>]. <notation>
  <usage><m>G</m></usage>
  <description>universal gravitational constant</description>
</notation>
    </p>
   </introduction>

   <subsection xml:id="subsec-accl_grav">
    <title>Acceleration Due to Gravity, <m>g</m> </title>
    <figure xml:id="NLG2">
      <caption></caption>
      <image source="NLG2.png" width="20%"/>
  </figure>
   <introduction>
    <p>
        From Newton's II law of motion, when an external unbalanced force acts on an object, 
        it will give  an acceleration <m>a</m> to that object, that is, <m>F = ma</m>. 
        But, if the gravitational force is acting on the body near the surface of the earth, 
        then the body experiences the acceleration <m>g</m> for a freely falling body. 
        This force is called weight of the body, <m>w = mg</m>. Hence, 
        <me>
          F=mg=G\frac{Mm}{R^{2}} \quad \Rightarrow\quad g=\frac{GM}{R^{2}} 
        </me>
        Where <m>M, \quad m,</m> and <m>R</m> are the mass of earth, mass of a body on the 
        surface of the earth, and the radius of the earth, respectively. The shape of 
        earth is not a perfect sphere, rather, it is an oblate spheroid. That is, 
        the radius of the earth at the equator <m> R_{eq}</m> is slightly greater 
        than the radius of the earth at the poles <m>R_{pol}</m> as shown in 
        <xref ref="NLG1"/>. Hence the value of <m>g</m> varies slightly with  latitude 
        on the surface of the earth as <m>g \varpropto \frac{1}{R^{2}},</m> since G and M 
        are constants. The value of 
        <me>
          R_{pol}=6.356\times10^{6}m, \quad R_{eq} = 6.378\times10^{6}m, 
        </me>
       The mean value of <m>R = 6.371\times10^{6}m.</m> Even though the variation in 
       the radius of the earth seems quite small, the variation in the acceleration 
       due to gravity on the earth goes from as low as <m>9.78 m/s^{2}</m> at the equator 
       to as high as <m>9.83 m/s^{2}</m> at the north Pole.
      </p>
    </introduction>


    <subsubsection xml:id="subsubsec-rot_g">
      <title>Effect of the Rotation of the Earth on  g</title>
      <figure xml:id="NLG3">
        <caption></caption>
        <image source="NLG3.png" width="35%"/>
    </figure>
      <p>
        The value of <m>g</m> on the surface of the earth does not only vary with the 
        radius of the earth but it is also affected by the rotation of the earth. Any 
        mass rotating in a circular motion needs a centripetal force which is acting towards 
        the center of the circular path. Remember that a centripetal force is not a real 
        force that is acting on a rotating body, but it is the required force that must be 
        applied to keep the body in that rotational motion. Hence the part of gravitational 
        force must be acting on a body to provide a necessary centripetal force to keep 
        that object moving on a circle with the rotation of the earth as shown in <xref ref="NLG3"/>. 
      </p>
      <p>
        Since the centripetal force <m>\vec{F}_{c}=m\vec{a}_{c}</m> required by the mass 
        m to follow a circle of radius r, then this force must be provided by the 
        vector difference in force of gravity <m>\vec{F_{e}}=m\vec{g}_{e} </m> and 
        a real force <m>F=m\vec{g}</m>, i.e., 
        <me>
          \vec{F}_{c}=\vec{F_{e}}-\vec{F} 
        </me>
        <me>
          \text{or,}\quad m\vec{a}_{c} = m\vec{g}_{e}-m\vec{g} 
        </me>
        <me>
          \therefore \vec{g}=\vec{g}_{e}-\vec{a}_{c}
        </me>
       The magnitude of <m>\vec{g}</m> can be found by 
       <me>
        \vec{g}\cdot\vec{g} =g^{2}= \left(\vec{g}_{e}-\vec{a}_{c}\right) \cdot\left(\vec{g}_{e}-\vec{a}_{c}\right)
       </me>
       <me>
        = \vec{g}_{e}\cdot\vec{g}_{e} + \vec{a}_{c}\cdot\vec{a}_{c}-2\vec{g}_{e}\cdot\vec{a}_{c} =g^{2}_{e}+a^{2}_{c}-2g_{e}a_{c}\cos\lambda 
       </me>
       <me>
        \therefore g= \sqrt{g^{2}_{e}+a^{2}_{c}-2g_{e}a_{c}\cos\lambda} 
       </me>
       where <me>
        a_{c}=r\omega^{2} = R\omega^{2}\cos\lambda,
      </me> 
        R is the radius of the earth, and the acceleration due to gravity on a non-rotating earth is
       <me>
        g_{e}= \frac{GM}{R^{2}}.
       </me>
      </p>
    </subsubsection>

<subsubsection xml:id="subsubsec-alt_g">
  <title>Effect of Altitude of the Earth on g</title>
  <figure xml:id="NLG4">
    <caption></caption>
    <image source="NLG4.png" width="35%"/>
</figure>
  <p>
    Acceleration due to gravity on the surface of the earth is given by  
    <me>
      g=\frac{GM}{R^{2}}
    </me>
   At height <m>h</m> from the surface of the earth [Figure <xref ref="NLG4"/>],  
   acceleration due to gravity is given by 
   <me>
    g_{h} = \frac{GM}{(R+h)^{2}} = \frac{GM}{R^{2}\left(1+\frac{h}{R}\right)^{2}}
   </me>
   <me>
    =\frac{g}{\left(1+\frac{h}{R}\right)^{2}}=g\left(1+\frac{h}{R}\right)^{-2} =g\left(1-\frac{2h}{R} +\cdots\right)
   </me>
   using binomial theorem
   <me>
    \therefore \quad g_{h} =g\left(1-\frac{2h}{R}\right)
   </me>
     </p>
</subsubsection>

<subsubsection xml:id="subsubsec-depth_g">
  <title>Effect of Depth of the Earth on g</title>
  <figure xml:id="NLG5">
    <caption></caption>
    <image source="NLG5.png" width="35%"/>
</figure>
  <p>
    Acceleration due to gravity on the surface of the earth is given by 
    <me>
      g=\frac{GM}{R^{2}}= \frac{G}{R^{2}}\left(\frac{4}{3}\pi R^{3}\rho\right) = \frac{4}{3}G\pi R\rho
    </me>
    where mass of the entire earth, 
    <me>
      M=Volume\times density = \left(\frac{4}{3}\pi R^{3}\right)\times \rho
    </me>
   At depth <m>d</m> from the surface of the earth, mass of the earth 
   <me>
    M'=\frac{4}{3}\pi (R-d)^{3} \rho
   </me>
    [<xref ref="NLG5"/>]. Therefore the acceleration due to gravity at that depth is given by
    <me>
      g_{d} = \frac{GM'}{(R-d)^{2}} = \frac{\frac{4}{3}G\pi (R-d)^{3} \rho}{(R-d)^{2}} 
    </me>
    <me>
      =\frac{4}{3}G\pi (R-d) \rho = \frac{4}{3}G\pi \rho R\left(1-\frac{d}{R}\right) 
    </me>
    <me>
      \therefore \quad g_{h} =g\left(1-\frac{d}{R}\right)
    </me>
   </p>
</subsubsection>
   </subsection>


   <subsection xml:id="subsec-grav_pot">
    <title>Gravitational Potential Energy, U</title>
    <figure xml:id="NLG6">
      <caption></caption>
      <image source="NLG6.png" width="35%"/>
  </figure>
    <p>
      The gravitational potential energy of a body is work required to bring 
      that body from infinity to the particular position in a gravitational field. 
      Let a body of mass <m>m</m> is displaced without acceleration by a distance 
      <m>\,dr</m> against the force of gravity, then work done by the external force 
      <m>\vec{F}_{r}</m> is given by
      <me>
        \,dw=\vec{F}_{r}\cdot\,d\vec{r} = F_{r}\,dr = G\frac{Mm}{r^{2}}\,dr 
      </me>
         If a body is displaced from a position <m>A</m> of distance <m>r_{1}</m> 
          to a position <m>B</m> at distance <m>r_{2}</m> against the gravity [<xref ref="NLG6"/>], then 
          <me>
            W=\int\,dw=\int\limits_{r_{1}}^{r_{2}} G\frac{Mm}{r^{2}}\,dr
          </me>
          <me>
            = -GMm\left(\frac{1}{r}\right)_{r_{1}}^{r_{2}} =-GMm \left(\frac{1}{r_{2}}-\frac{1}{r_{1}}\right)
          </me>
          Hence work done by the gravity, (or the gravitational potential energy) is given by 
          <me>
            U= -W = GMm \left(\frac{1}{r_{2}}-\frac{1}{r_{1}}\right)
          </me>
If a body is brought from infinity to any point at a distance <m>r</m> in the gravitational field then, 
<me>
  U(r) = GMm \left(\frac{1}{\infty}-\frac{1}{r}\right) = -\frac{GMm}{r} 
</me>
In calculus form, potential energy is defined as
<me>
  U(r) = -\int\limits_{\infty}^{r}F_{r}\cdot\,dr
</me>
where <m>F_{r}</m> is a conservative foece, and therefore force can be written as 
<me>
  F_{r}=-\frac{\,dU}{\,dr}.
</me>
          </p>
   </subsection>

   <subsection xml:id="subsec-orb_vel">
    <title>Orbital Velocity of a Satelite</title>
    <figure xml:id="NLG7">
      <caption></caption>
      <image source="NLG7.png" width="35%"/>
  </figure>
    <p>
      The velocity of a satellite in its orbit around the planet is called the orbital velocity, 
      <m>v_{o}</m>. To move in a circular track an object must need a centripetal force 
      which is provided by the force of gravity between the object and the planet. i.e.,
      <me>
        F_{c} = F_{g} \quad \Rightarrow\quad \frac{mv^{2}_{o}}{r}=G\frac{Mm}{r^{2}}
      </me>
      <me>
        \therefore v_{o} = \sqrt{\frac{GM}{r}} =\sqrt{\frac{GM}{R+h}}
      </me>
      Where <m>r=R+h </m>, <m>m</m>, and <m>M</m> are distance of a satellite (object), 
      mass of a satellite, and mass of the planet, respectively. <m>R</m> is radius of the planet, 
      <m>G</m> is universal gravitational constant, and <m>h</m> is the altitude of the 
      satellite from the surface of the planet.
    </p>
   </subsection>

   <subsection xml:id="subsec-esc_vel">
    <title>Escape Velocity</title>
    <figure xml:id="NLG8">
      <caption></caption>
      <image source="NLG8.png" width="35%"/>
  </figure>
    <p>
      The minimum velocity of an object with which it can be thrown out from 
      the planet so that it never come back is known as escape velocity. 
      Suppose a stone of mass <m>m</m> is thrown out from a planet with a velocity <m>v_{e}</m> 
       so that it never fall back on the earth again, then the total energy of the 
       stone on the planet, <m>E_{p}</m> is equal to total energy of the stone at infinity, <m>E_{\infty}. </m>
       <me>
        E_{p} = E_{\infty} \quad \Rightarrow\quad KE_{p} + PE_{p} =KE_{\infty}+PE_{\infty}
       </me>
       <me>
        \frac{mv^{2}_{e}}{2}-\frac{GMm}{R} = 0-\frac{GMm}{\infty} 
       </me>
       <me>
        \therefore v_{e} = \sqrt{\frac{2GM}{R}}
       </me>
       Where <m>r=R+h</m>, <m>m</m>, and <m>M</m> are distance of a satellite (object), 
       mass of a satellite, and mass of the planet, respectively. Here <m>R</m> is radius 
       of the planet,  <m>G</m> is universal gravitational constant, and <m>h</m> is the 
       altitude of the satellite from the surface of the planet. 
       If radius of the earth, <m>R=6.37\times10^{6}m</m>  and mass of the earth is <m>M=5.97\times10^{24}kg</m>, then
       <me>
        v_{e} = \sqrt{\frac{2\times 6.67\times10^{-11}\times5.97\times10^{24}}{6.37\times10^{6}}} 
       </me>
       <me>
        \therefore \quad  v_{e} =1.12\times10^{4}m/s= 11.2km/s.
       </me>
           </p>
   </subsection>

   <subsection xml:id="subsec-geo_sync">
    <title>Geosynchronous satellite</title>
    <figure xml:id="NLG9">
      <caption></caption>
      <image source="NLG9.png" width="35%"/>
  </figure>
    <p>
      A geosynchronous satellite orbits the earth in such a way that it reaches 
      at the same point above the earth in every 24 hours. The special kind of geosynchronous 
      satellite is called geostationary satellite 
      which seems to be at rest at the same position above the earth. Geostationary satellite takes an equatorial 
      orbit. The geosynchronous satellite orbits in such a way that it seems shifting from north to south about an equatorial orbit 
      but due to earth orientation and rotation. Some sattelites also revolve along polar orbit. Polar satellites 
      can be useful in weather forecasting and mapping the globe. Geostationary satellite are used for long term weather forecasting, spying,
      communications, broadcasting, and signal transmission.  
    </p>
      <p>
      The necessary centripetal force of such satellite is given by the gravitational force. 
           <men xml:id="eqn-geosync1">
        F_{g}=\frac{GMm}{r^{2}} = \frac{mv^{2}_{o}}{r}
      </men>
      Where <m>m,</m> <m>v_{o},</m> and <m>r</m> are mass, orbital velocity, 
      and the orbital radius of the  satellite, respectively. Also 
      <men xml:id="eqn-geosync2">
        v_{o} = \frac{2\pi r}{T} 
      </men>
      Where <m>T</m> is orbiting time period of satellite. From eqns. 
      <xref ref="eqn-geosync1"/> and <xref ref="eqn-geosync2"/>, we have -
      <men xml:id="eqn-geosync3">
        r =\sqrt[3]{\frac{GMT^{2}}{4\pi^{2}}}
      </men>
      Since the angular speed of satellite in its orbit must be the same as that of the 
      earth about its axis, the orbiting time period of satellite must be equal to 1 day. 
      Therefore,  
      <me>
        T = 1 day = 24 h \times 60 \frac{min}{h}\times 60 \frac{sec}{min} = 86400 s
      </me>
      <me>
        \therefore \quad r=4.23\times10^{7} m
      </me>
           A geostationary satellite must orbit at a distance of about 36000 km 
           above the surface of the earth, [<m>\because\quad r=R+h</m>].
         </p>
   </subsection>
  </section>

